<?xml version="1.0" encoding="UTF-8"?>

<section xml:id="sec-the-lagrangian-functions">
  <title>The Lagrangian function</title>

  <objectives>
    <ol>
      <li>
        <p>
          
        </p>
      </li>
      <li>
        <p>
          
        </p>
      </li>
      <li>
        <p>
          
        </p>
      </li>
    </ol>
  </objectives>
  
  <introduction>
    <p>
      Introduction goes here.
    </p>
  </introduction>

  <ul>
    <li>
      <p>
        <url href="http://www.slimy.com/~steuard/teaching/tutorials/Lagrange.html">http://www.slimy.com/~steuard/teaching/tutorials/Lagrange.html</url>
      </p>
    </li>

    <li>
      <p>
        Here's another way we can “zoom out” and see the Lagrange multiplier method as part of a bigger story.
      </p>
    </li>

    <li>
      <p>
        Suppose we want to maximize <m>f(x,y)</m> subject to the constraint <m>g(x,y)=c</m>.
        Define the Lagrangian function:
        <me>
          \cl{L}(x,y,\lambda)=f(x,y)+\lambda(c-g(x,y))
        </me>
        <me>
          \cl{L}=f+\lambda(c-g)
        </me>
        Then the solution to our maximization problem is the point where <m>\Grad\cl{L}=0</m>:
      </p>
      <md>
        <mrow>\pdv{f}{x} - \lambda\pdv{g}{x} \amp = 0</mrow>
        <mrow>\pdv{f}{y} - \lambda\pdv{g}{y} \amp = 0</mrow>
        <mrow>c - g(x,y) \amp = 0</mrow>
      </md>

      <p>
        Note that we're assuming that <m>c</m> is a constant for now.
      </p>
    </li>

    <li>
      <p>
        Note that <m>\DS\pdv{\cl{L}}{c}=\lambda</m>, which means that <m>\lambda</m> represents the sensitivity of the Lagrangian function to changes in our constraint amount.
        It can also be shown (will have to look at how!) that <m>\DS\pdv{\cl{L}}{c}=\pdv{f}{c}</m>; apparently this uses the “envelope theorem.”
      </p>
    </li>

    <li>
      <p>
        Let <m>(x^{*},y^{*})</m> be the solution to the constrained optimization problem.
        This depends on the given value of <m>c</m>, so we'll write them as <m>(x^{*}(c),y^{*}(c))</m>, and we'll write the optimum value of <m>f</m> here as
        <me>
          f(x^{*}(c),y^{*}(c))
        </me>.
        If we differentiate with respect to <m>c</m>, we get:
        <me>
          \dv{f}{c}=\pdv f{x^*}\dv{x^*}{c}+\pdv f{y^*}\dv{y^*}{c}
        </me>
        Additionally, the constraint satisfies the equation
        <me>
          g(x^{*}(c),y^{*}(c))=c
        </me>.
        Differentiate both sides with respect to <m>c</m> using the Chain Rule:
        <me>
          \pdv g{x^*}\dv{x^*}{c}+\pdv g{y^*}\dv{y^*}{c}=1
        </me>
        By the Lagrange multiplier property we know that:
        <me>
          \Grad f=\lambda\Grad g
        </me>
        Taking dot products with <m>\DS\dd{\bv{r}}^{*}=\qty(\dv{x^*}{c},\dv{y^*}{c})</m>:
        <me>
          \Grad f\cdot\dd{\bv{r}}^{*}=\lambda\Grad g\cdot\dd{\bv{r}}^{*}
        </me>
        Since <m>\Grad g\cdot\dd{\bv{r}}^{*}=1</m> we have:
        <me>
          \dv{f}{c}=\lambda
        </me>
      </p>
    </li>

    <li>
      <p>
        Might actually be able to tie this to holding certain variables constant in <m>\cl{L}(x,y,\lambda,c)</m>, à la thermodynamics notation.
      </p>
    </li>
  </ul>
</section>
